Begin new approach recording rightmost error for successful parses
This is important for things like repetition-forms.  For example, if
you have a FOO non-terminal and attempt to parse (rpt FOO) in a
context where there is a line of input which looks like a FOO right up
to character 60 and then causes the FOO to fail.  The current approach
would have the rpt succeed at the start of the input with nothing
consumed.  This then leads to very unhelpful error-reporting.

Committing because I am going to go back and get rid of locs; I need
these to be monotonically increasing so I now want the peg engine to
track these numbers/locations itself.

examples/formal-languages/context-free/pegScript.sml
@@ -33,24 +33,24 @@ Datatype:
 End
 
 Datatype:
-  pegresult = Success 'a 'c
+  pegresult = Success 'a 'c ((locs # 'e) option)
             | Failure locs 'e
 End
 Definition isSuccess_def[simp]:
-  isSuccess (Success _ _) = T ∧
+  isSuccess (Success _ _ _) = T ∧
   isSuccess (Failure _ _) = F
 End
 Definition isFailure_def[simp]:
-  isFailure (Success _ _) = F ∧
+  isFailure (Success _ _ _) = F ∧
   isFailure (Failure _ _) = T
 End
 
 Definition resultmap_def[simp]:
-  resultmap f (Success a c) = Success a (f c) ∧
+  resultmap f (Success a c eo) = Success a (f c) eo ∧
   resultmap f (Failure fl fe) = Failure fl fe
 End
 Theorem resultmap_EQ_Success :
-  resultmap f r = Success a x ⇔ ∃x0. r = Success a x0 ∧ x = f x0
+  resultmap f r = Success a x eo ⇔ ∃x0. r = Success a x0 eo ∧ x = f x0
 Proof
   Cases_on ‘r’ >> simp[] >> metis_tac[]
 QED
@@ -61,19 +61,20 @@ Theorem resultmap_EQ_Failure[simp]:
 Proof
   Cases_on ‘r’ >> simp[] >> metis_tac[]
 QED
-Definition rmax_def[simp]:
-  rmax (Success a c) _ = Success a c ∧
-  rmax (Failure _ _) (Success a c) = Success a c ∧
-  rmax (Failure fl1 fe1) (Failure fl2 fe2) =
-  if locsle fl1 fl2 then Failure fl2 fe2 else Failure fl1 fe1
+
+Definition MAXerr_def:
+  MAXerr (fl1, fe1) (fl2, fe2) =
+  if locsle fl1 fl2 then (fl2, fe2) else (fl1,fe1)
 End
 
-Theorem rmax_EQ_Success:
-  rmax r1 r2 = Success x y ⇔
-  r1 = Success x y ∨ r2 = Success x y ∧ isFailure r1
-Proof
-  Cases_on ‘r1’ >> simp[] >> Cases_on ‘r2’ >> simp[AllCaseEqs()]
-QED
+Definition optmax_def:
+  optmax f NONE NONE = NONE ∧
+  optmax f NONE (SOME x) = SOME x ∧
+  optmax f (SOME x) NONE = SOME x ∧
+  optmax f (SOME x) (SOME y) = SOME (f x y)
+End
+
+
 
 Theorem result_cases[local] = TypeBase.nchotomy_of “:(α,β,γ) pegresult”
 
@@ -91,80 +92,114 @@ QED
 
 (* Option type should be replaced with sum type (loc. for NONE *)
 Inductive peg_eval:
-  (∀s c. peg_eval G (s, empty c) (Success s c)) ∧
+[~empty:]
+  (∀s c. peg_eval G (s, empty c) (Success s c NONE)) ∧
+[~nt_success:]
   (∀n r s f c.
-       n ∈ FDOM G.rules ∧ peg_eval G (s, G.rules ' n) (Success r c) ⇒
-       peg_eval G (s, nt n f) (Success r (f c))) ∧
+       n ∈ FDOM G.rules ∧ peg_eval G (s, G.rules ' n) (Success r c eo) ⇒
+       peg_eval G (s, nt n f) (Success r (f c) eo)) ∧
+[~nt_failure:]
   (∀n s f fe fl.
        n ∈ FDOM G.rules ∧ peg_eval G (s, G.rules ' n) (Failure fl fe) ⇒
        peg_eval G (s, nt n f) (Failure fl fe)) ∧
-  (∀h t f. peg_eval G (h::t, any f) (Success t (f h))) ∧
+[~any_success:]
+  (∀h t f. peg_eval G (h::t, any f) (Success t (f h) NONE)) ∧
+[~any_failure:]
   (∀f. peg_eval G
                 ([] : ('a # locs) list, any f)
                 (Failure (sloc ([] : ('a # locs) list)) G.anyEOF)) ∧
-  (∀e t P f. P (FST e) ⇒ peg_eval G (e::t, tok P f) (Success t (f e))) ∧
+[~tok_success:]
+  (∀e t P f. P (FST e) ⇒ peg_eval G (e::t, tok P f) (Success t (f e) NONE)) ∧
+[~tok_failureF:]
   (∀e t P f.
      ¬P (FST e) ⇒
      peg_eval G (e::t, tok P f) (Failure (sloc (e::t)) G.tokFALSE)) ∧
+[~tok_failureEOF:]
   (∀P f. peg_eval G ([], tok P f)
                   (Failure (sloc ([] : ('a # locs) list)) G.tokEOF)) ∧
+[~not_success:]
   (∀e s c fr.
      peg_eval G (s, e) fr ∧ isFailure fr ⇒
-     peg_eval G (s, not e c) (Success s c)) ∧
+     peg_eval G (s, not e c) (Success s c NONE)) ∧
+[~not_failure:]
   (∀e s r c.
      peg_eval G (s, e) r ∧ isSuccess r ⇒
      peg_eval G (s, not e c) (Failure (sloc s) G.notFAIL))  ∧
+[~seq_fail1:]
   (∀e1 e2 s f fr.
      peg_eval G (s, e1) fr ∧ isFailure fr ⇒ peg_eval G (s, seq e1 e2 f) fr)  ∧
-  (∀e1 e2 s0 s1 c1 fr.
-     peg_eval G (s0, e1) (Success s1 c1) ∧
-     peg_eval G (s1, e2) fr ∧ isFailure fr ⇒
-     peg_eval G (s0, seq e1 e2 f) fr) ∧
+[~seq_fail2:]
+  (∀e1 e2 s0 eo s1 c1 fl fe.
+     peg_eval G (s0, e1) (Success s1 c1 eo) ∧
+     peg_eval G (s1, e2) (Failure fl fe) ⇒
+     peg_eval G (s0, seq e1 e2 f) (Failure fl fe)) ∧
+[~seq_success:]
   (∀e1 e2 s0 s1 s2 c1 c2 f.
-     peg_eval G (s0, e1) (Success s1 c1) ∧
-     peg_eval G (s1, e2) (Success s2 c2) ⇒
-     peg_eval G (s0, seq e1 e2 f) (Success s2 (f c1 c2))) ∧
-  (∀e1 e2 s f f1 f2.
-     peg_eval G (s, e1) f1  ∧ peg_eval G (s, e2) f2 ∧
-     isFailure f1 ∧ isFailure f2 ⇒
-     peg_eval G (s, choice e1 e2 f) (rmax f1 f2)) ∧
-  (∀e1 e2 s f sr.
-     peg_eval G (s, e1) sr ∧ isSuccess sr ⇒
-     peg_eval G (s, choice e1 e2 f) (resultmap (f o INL) sr)) ∧
-  (∀e1 e2 s f fr sr.
-     peg_eval G (s, e1) fr ∧ isFailure fr ∧
-     peg_eval G (s, e2) sr ∧ isSuccess sr ⇒
-     peg_eval G (s, choice e1 e2 f) (resultmap (f o INR) sr)) ∧
+     peg_eval G (s0, e1) (Success s1 c1 eo1) ∧
+     peg_eval G (s1, e2) (Success s2 c2 eo2) ⇒
+     peg_eval G (s0, seq e1 e2 f)
+              (Success s2 (f c1 c2) (optmax MAXerr eo1 eo2))) ∧
+[~choice_fail:]
+  (∀e1 e2 s f fl1 fe1 fl2 fe2.
+     peg_eval G (s, e1) (Failure fl1 fe1) ∧
+     peg_eval G (s, e2) (Failure fl2 fe2) ⇒
+     peg_eval G (s, choice e1 e2 f)
+              (UNCURRY Failure (MAXerr (fl1,fe1) (fl2,fe2)))) ∧
+[~choice_success1:]
+  (∀e1 e2 s0 f s r eo.
+     peg_eval G (s0, e1) (Success s r eo) ⇒
+     peg_eval G (s0, choice e1 e2 f) (Success s (f (INL r)) eo)) ∧
+[~choice_success2:]
+  (∀e1 e2 s0 s r eo f fl fe.
+     peg_eval G (s0, e1) (Failure fl fe) ∧
+     peg_eval G (s0, e2) (Success s r eo) ⇒
+     peg_eval G (s0, choice e1 e2 f)
+              (Success s (f (INR r)) (optmax MAXerr (SOME (fl,fe)) eo))) ∧
+[~error:]
   (∀e s. peg_eval G (s, error e) (Failure (sloc s) e)) ∧
 [~rpt:]
   (∀e f s s1 list.
-     peg_eval_list G (s, e) (s1,list) ⇒
-     peg_eval G (s, rpt e f) (Success s1 (f list))) ∧
+     peg_eval_list G (s, e) (s1,list,err) ⇒
+     peg_eval G (s, rpt e f) (Success s1 (f list) (SOME err))) ∧
 [~list_nil:]
-  (∀e s fr. peg_eval G (s, e) fr ∧ isFailure fr ⇒
-            peg_eval_list G (s, e) (s,[])) ∧
+  (∀e s fl fe. peg_eval G (s, e) (Failure fl fe) ⇒
+               peg_eval_list G (s, e) (s,[],(fl,fe))) ∧
 [~list_cons:]
-  (∀e s0 s1 s2 c cs.
-     peg_eval G (s0, e) (Success s1 c) ∧
-     peg_eval_list G (s1, e) (s2,cs) ⇒
-     peg_eval_list G (s0, e) (s2,c::cs))
+  (∀e eo0 eo s0 s1 s2 c cs.
+     peg_eval G (s0, e) (Success s1 c eo0) ∧
+     peg_eval_list G (s1, e) (s2,cs,eo) ⇒
+     peg_eval_list G (s0, e) (s2,c::cs,eo))
 End
 
+val fprod = HO_REWR_CONV pairTheory.FORALL_PROD
 Theorem peg_eval_strongind' =
   peg_eval_strongind
-    |> SIMP_RULE (srw_ss()) [pairTheory.FORALL_PROD]
     |> Q.SPECL [`G`, `\es0 r. P1 (FST es0) (SND es0) r`,
-                `\es0 sr. P2 (FST es0) (SND es0) (FST sr) (SND sr)`]
+                `\es0 sr. P2 (FST es0) (SND es0) (FST sr) (FST $ SND sr)
+                (SND $ SND sr)`]
     |> SIMP_RULE (srw_ss()) []
+    |> UNDISCH |> CONJ_PAIR
+    |> (SIMP_RULE (srw_ss()) [pairTheory.FORALL_PROD] ##
+        CONV_RULE (fprod THENC
+                   LAST_FORALL_CONV (fprod THENC LAST_FORALL_CONV fprod)))
+    |> uncurry CONJ
+    |> SIMP_RULE (srw_ss()) []
+    |> DISCH_ALL;
+
+Theorem UNCURRY_Failure_EQ_Success[simp]:
+  UNCURRY Failure fle ≠ Success s r eo
+Proof
+  Cases_on ‘fle’ >> simp[]
+QED
 
 open rich_listTheory
 Theorem peg_eval_suffix0[local]:
-  (∀s0 e sr. peg_eval G (s0,e) sr ⇒ ∀s r. sr = Success s r ⇒ IS_SUFFIX s0 s) ∧
-  ∀s0 e s rl. peg_eval_list G (s0,e) (s,rl) ⇒ IS_SUFFIX s0 s
+  (∀s0 e sr. peg_eval G (s0,e) sr ⇒
+             ∀s r eo. sr = Success s r eo ⇒ IS_SUFFIX s0 s) ∧
+  ∀s0 e s rl err. peg_eval_list G (s0,e) (s,rl,err) ⇒ IS_SUFFIX s0 s
 Proof
   HO_MATCH_MP_TAC peg_eval_strongind' THEN
   SRW_TAC [][IS_SUFFIX_compute, IS_PREFIX_APPEND3, IS_PREFIX_REFL] THEN
-  fs[rmax_EQ_Success, resultmap_EQ_Success] >>
   METIS_TAC [IS_PREFIX_TRANS]
 QED
 
@@ -175,27 +210,25 @@ Theorem peg_eval_suffix =
 (* Theorem 3.2 *)
 Theorem peg_deterministic:
   (∀s0 e sr. peg_eval G (s0,e) sr ⇒ ∀sr'. peg_eval G (s0,e) sr' ⇔ sr' = sr) ∧
-  ∀s0 e s rl. peg_eval_list G (s0,e) (s,rl) ⇒
-              ∀srl'. peg_eval_list G (s0,e) srl' ⇔ srl' = (s,rl)
+  ∀s0 e s rl err. peg_eval_list G (s0,e) (s,rl,err) ⇒
+                  ∀srl'. peg_eval_list G (s0,e) srl' ⇔ srl' = (s,rl,err)
 Proof
   HO_MATCH_MP_TAC peg_eval_strongind' THEN SRW_TAC [][] THEN
   ONCE_REWRITE_TAC [peg_eval_cases] THEN SRW_TAC [][] THEN
+  csimp[] >>
   TRY (Q.MATCH_ASSUM_RENAME_TAC ‘isSuccess result’ >>
        Cases_on ‘result’ >> fs[]) THEN
   TRY (Q.MATCH_ASSUM_RENAME_TAC ‘isFailure result’ >>
-       Cases_on ‘result’ >> fs[]) THEN csimp[] THEN
-  Q.MATCH_ASSUM_RENAME_TAC ‘isFailure result2’ >> Cases_on ‘result2’ >> fs[]
+       Cases_on ‘result’ >> fs[])
 QED
 
 (* Lemma 3.3 *)
 Theorem peg_badrpt:
-  peg_eval G (s0,e) (Success s0 r) ⇒ ∀r. ¬peg_eval G (s0, rpt e f) r
+  peg_eval G (s0,e) (Success s0 r eo) ⇒ ∀r. ¬peg_eval G (s0, rpt e f) r
 Proof
-  strip_tac >> simp[Once peg_eval_cases] >> map_every qx_gen_tac [`s1`, `l`] >>
-  disch_then (assume_tac o MATCH_MP (CONJUNCT2 peg_deterministic)) >>
-  `peg_eval_list G (s0,e) (s1,r::l)`
-    by METIS_TAC [last (peg_eval_rules |> SPEC_ALL |> CONJUNCTS)] >>
-  pop_assum mp_tac >> simp[]
+  strip_tac >> simp[Once peg_eval_cases] >>
+  rpt strip_tac >> dxrule_then assume_tac $ cj 2 peg_deterministic  >>
+  drule peg_eval_list_cons >> simp[]
 QED
 
 Inductive peg0:
@@ -252,8 +285,8 @@ Proof
 QED
 
 Theorem peg_eval_suffix':
-  peg_eval G (s0,e) (Success s c) ⇒
-  s0 = s ∨ IS_SUFFIX s0 s ∧ LENGTH s < LENGTH s0
+peg_eval G (s0,e) (Success s c eo) ⇒
+        s0 = s ∨ IS_SUFFIX s0 s ∧ LENGTH s < LENGTH s0
 Proof
   strip_tac >> imp_res_tac peg_eval_suffix >> Cases_on `s0 = s` >- simp[] >>
   fs[IS_SUFFIX_compute] >>
@@ -264,8 +297,8 @@ Proof
 QED
 
 Theorem peg_eval_list_suffix':
-  peg_eval_list G (s0, e) (s,rl) ⇒
-  s0 = s ∨ IS_SUFFIX s0 s ∧ LENGTH s < LENGTH s0
+peg_eval_list G (s0, e) (s,rl,err) ⇒
+        s0 = s ∨ IS_SUFFIX s0 s ∧ LENGTH s < LENGTH s0
 Proof
   strip_tac >> imp_res_tac peg_eval_suffix >> Cases_on `s0 = s` >- simp[] >>
   fs[IS_SUFFIX_compute] >> imp_res_tac IS_PREFIX_LENGTH >> fs[] >>
@@ -274,28 +307,28 @@ Proof
 QED
 
 fun rule_match th = FIRST (List.mapPartial (total MATCH_MP_TAC)
-                                           (th |> SPEC_ALL |> CONJUNCTS))
+                           (th |> SPEC_ALL |> CONJUNCTS))
 
 Theorem FORALL_result:
-  (∀r. P r) ⇔ (∀a c. P (Success a c)) ∧ (∀fl fe. P (Failure fl fe))
+  (∀r. P r) ⇔ (∀a c eo. P (Success a c eo)) ∧ (∀fl fe. P (Failure fl fe))
 Proof
   rw[EQ_IMP_THM] >> Cases_on ‘r’ >> simp[]
 QED
 
 Theorem EXISTS_result:
-  (∃r. P r) ⇔ (∃a c. P (Success a c)) ∨ (∃fl fe. P (Failure fl fe))
+  (∃r. P r) ⇔ (∃a c eo. P (Success a c eo)) ∨ (∃fl fe. P (Failure fl fe))
 Proof
   rw[EQ_IMP_THM] >- (Cases_on ‘r’ >> metis_tac[]) >> metis_tac[]
 QED
 
 Theorem lemma4_1a0[local]:
   (∀s0 e r. peg_eval G (s0, e) r ⇒
-            (∀c. r = Success s0 c ⇒ peg0 G e) ∧
+            (∀c eo. r = Success s0 c eo ⇒ peg0 G e) ∧
             (isFailure r ⇒ pegfail G e) ∧
-            (∀s c. r = Success s c ∧ LENGTH s < LENGTH s0 ⇒ peggt0 G e)) ∧
-  (∀s0 e s rl. peg_eval_list G (s0,e) (s,rl) ⇒
-               (s0 = s ⇒ pegfail G e) ∧
-               (LENGTH s < LENGTH s0 ⇒ peggt0 G e))
+            (∀s c eo. r = Success s c eo ∧ LENGTH s < LENGTH s0 ⇒ peggt0 G e)) ∧
+  (∀s0 e s rl err. peg_eval_list G (s0,e) (s,rl,err) ⇒
+                   (s0 = s ⇒ pegfail G e) ∧
+                   (LENGTH s < LENGTH s0 ⇒ peggt0 G e))
 Proof
   ho_match_mp_tac peg_eval_strongind' >> simp[peg0_rules, FORALL_result] >>
   rpt conj_tac
@@ -305,8 +338,7 @@ Proof
       full_simp_tac (srw_ss() ++ ARITH_ss) [])
   >- (rpt strip_tac >> rule_match peg0_rules >>
       imp_res_tac peg_eval_suffix' >> fs[] >> rw[] >>
-      full_simp_tac (srw_ss() ++ ARITH_ss) [])
-  >- simp[AllCaseEqs()] >>
+      full_simp_tac (srw_ss() ++ ARITH_ss) []) >>
   rpt strip_tac
   >- (first_x_assum match_mp_tac >> rw[] >>
       imp_res_tac peg_eval_suffix >> fs[IS_SUFFIX_compute] >>
@@ -395,14 +427,14 @@ val list_CASES = listTheory.list_CASES
 
 Theorem reducing_peg_eval_makes_list[local]:
   (∀s. LENGTH s < n ⇒ ∃r. peg_eval G (s, e) r) ∧ ¬peg0 G e ∧ LENGTH s0 < n ⇒
-  ∃s' rl. peg_eval_list G (s0,e) (s',rl)
+  ∃s' rl err. peg_eval_list G (s0,e) (s',rl,err)
 Proof
   strip_tac >> completeInduct_on `LENGTH s0` >> rw[] >>
   full_simp_tac (srw_ss() ++ DNF_ss ++ ARITH_ss) [] >>
   ‘(∃fl fe. peg_eval G (s0,e) (Failure fl fe)) ∨
-   ∃s1 c. peg_eval G (s0,e) (Success s1 c)’
+   ∃s1 c eo. peg_eval G (s0,e) (Success s1 c eo)’
     by metis_tac [result_cases]
-  >- metis_tac [peg_eval_rules,isFailure_def, isSuccess_def] >>
+  >- metis_tac [peg_eval_list_nil] >>
   `s0 ≠ s1` by metis_tac [lemma4_1a] >>
   `LENGTH s1 < LENGTH s0` by metis_tac [peg_eval_suffix'] >>
   metis_tac [peg_eval_rules]
@@ -431,12 +463,12 @@ Proof
   >- (* any *) metis_tac [peg_eval_rules, list_CASES]
   >- (* tok *) metis_tac [peg_eval_rules, list_CASES]
   >- (* error *) metis_tac[peg_eval_rules]
-  >- (* not *) metis_tac [peg_eval_rules, result_cases, IN_Gexprs_E,
-                          isSuccess_def, isFailure_def]
+  >- (* not *) metis_tac [peg_eval_not_success, result_cases, IN_Gexprs_E,
+                          isFailure_def, isSuccess_def, peg_eval_not_failure]
   >- ((* seq *) rename [‘seq e1 e2 f ∈ Gexprs G’] >>
       ‘e1 ∈ Gexprs G’ by imp_res_tac IN_Gexprs_E >>
       ‘(∃fl fe. peg_eval G (s,e1) (Failure fl fe))  ∨
-       ∃s' c. peg_eval G (s,e1) (Success s' c)’
+       ∃s' c eo. peg_eval G (s,e1) (Success s' c eo)’
         by metis_tac[result_cases]
       >- metis_tac [peg_eval_rules, isFailure_def, isSuccess_def] >>
       Cases_on ‘s' = s’
@@ -452,11 +484,10 @@ Proof
      metis_tac [peg_eval_rules, result_cases, isSuccess_def, isFailure_def]) >>
   (* rpt *) imp_res_tac IN_Gexprs_E >>
   ‘(∃fl fe. peg_eval G (s, e) (Failure fl fe)) ∨
-   ∃s' c. peg_eval G (s,e) (Success s' c)’
+   ∃s' c eo. peg_eval G (s,e) (Success s' c eo)’
     by metis_tac [result_cases]
-  >- (‘peg_eval_list G (s,e) (s,[])’
-        by metis_tac [peg_eval_rules, isFailure_def] >>
-      metis_tac [peg_eval_rules]) >>
+  >- (‘peg_eval_list G (s,e) (s,[],fl,fe)’ by metis_tac [peg_eval_list_nil] >>
+      metis_tac [peg_eval_rpt]) >>
   ‘s' ≠ s’ by metis_tac [lemma4_1a] >>
   ‘LENGTH s' < LENGTH s’ by metis_tac [peg_eval_suffix'] >>
   metis_tac [peg_eval_rules, reducing_peg_eval_makes_list]
@@ -488,17 +519,19 @@ val checkAhead_def = Define`
 `;
 
 Theorem peg_eval_seq_SOME:
-  peg_eval G (i0, seq s1 s2 f) (Success i r) ⇔
-    ∃i1 r1 r2. peg_eval G (i0, s1) (Success i1 r1) ∧
-               peg_eval G (i1, s2) (Success i r2) ∧ (r = f r1 r2)
+  peg_eval G (i0, seq s1 s2 f) (Success i r eo) ⇔
+    ∃i1 r1 r2 eo1 eo2.
+      peg_eval G (i0, s1) (Success i1 r1 eo1) ∧
+      peg_eval G (i1, s2) (Success i r2 eo2) ∧ (r = f r1 r2) /\
+      eo = optmax MAXerr eo1 eo2
 Proof simp[Once peg_eval_cases] >> metis_tac[]
 QED
 
 Theorem peg_eval_seq_NONE:
   peg_eval G (i0, seq s1 s2 f) (Failure fl fe) ⇔
   peg_eval G (i0, s1) (Failure fl fe) ∨
-  ∃i r. peg_eval G (i0,s1) (Success i r) ∧
-        peg_eval G (i,s2) (Failure fl fe)
+  ∃i r eo. peg_eval G (i0,s1) (Success i r eo) ∧
+           peg_eval G (i,s2) (Failure fl fe)
 Proof
   simp[Once peg_eval_cases] >> metis_tac[]
 QED
@@ -508,19 +541,19 @@ Theorem peg_eval_tok_NONE =
     |> SIMP_CONV (srw_ss()) [Once peg_eval_cases]
 
 Theorem peg_eval_tok_SOME:
-  peg_eval G (i0, tok P f) (Success i r) ⇔
-  ∃h. P (FST h) ∧ i0 = h::i ∧ r = f h
+  peg_eval G (i0, tok P f) (Success i r eo) ⇔
+  ∃h. P (FST h) ∧ i0 = h::i ∧ r = f h ∧ eo = NONE
 Proof simp[Once peg_eval_cases] >> metis_tac[]
 QED
 
-Theorem peg_eval_empty[simp]: peg_eval G (i, empty r) x ⇔ x = Success i r
+Theorem peg_eval_empty[simp]: peg_eval G (i, empty r) x ⇔ x = Success i r NONE
 Proof simp[Once peg_eval_cases]
 QED
 
 Theorem peg_eval_NT_SOME:
-  peg_eval G (i0,nt N f) (Success i r) ⇔
+  peg_eval G (i0,nt N f) (Success i r eo) ⇔
   ∃r0. r = f r0 ∧ N ∈ FDOM G.rules ∧
-       peg_eval G (i0,G.rules ' N) (Success i r0)
+       peg_eval G (i0,G.rules ' N) (Success i r0 eo)
 Proof simp[Once peg_eval_cases]
 QED
 
@@ -529,14 +562,17 @@ Theorem peg_eval_choice:
      peg_eval G (i0, choice s1 s2 f) x ⇔
       (∃sr. peg_eval G (i0, s1) sr ∧ isSuccess sr ∧
             x = resultmap (f o INL) sr) ∨
-      (∃sr fr.
-         peg_eval G (i0, s1) fr ∧ isFailure fr ∧
-         peg_eval G (i0, s2) sr ∧ isSuccess sr ∧ x = resultmap (f o INR) sr) ∨
-      ∃fr1 fr2.
-        peg_eval G (i0, s1) fr1 ∧ peg_eval G (i0, s2) fr2 ∧
-        isFailure fr1 ∧ isFailure fr2 ∧ x = rmax fr1 fr2
+      (∃i r eo fl fe.
+         peg_eval G (i0, s1) (Failure fl fe) ∧
+         peg_eval G (i0, s2) (Success i r eo) ∧
+         x = Success i (f $ INR r) (optmax MAXerr (SOME (fl,fe)) eo)) ∨
+      ∃fl1 fe1 fl2 fe2.
+        peg_eval G (i0, s1) (Failure fl1 fe1) ∧
+        peg_eval G (i0, s2) (Failure fl2 fe2) ∧
+        x = UNCURRY Failure (MAXerr (fl1,fe1) (fl2,fe2))
 Proof
-  simp[Once peg_eval_cases, SimpLHS] >> metis_tac[]
+  simp[Once peg_eval_cases, SimpLHS] >> simp[EXISTS_result, FORALL_result] >>
+  metis_tac[]
 QED
 
 Theorem peg_eval_choicel_NIL[simp]:
@@ -547,30 +583,37 @@ QED
 
 Theorem peg_eval_choicel_CONS:
   ∀x. peg_eval G (i0, choicel (h::t)) x ⇔
-      peg_eval G (i0, h) x ∧ isSuccess x ∨
-      ∃fr ry.
-        peg_eval G (i0,h) fr ∧ isFailure fr ∧ peg_eval G (i0, choicel t) ry ∧
-        x = rmax fr ry
+        ∃y.
+          peg_eval G (i0, h) y ∧
+          case y of
+            Success i r eo => x = Success i r eo
+          | Failure fl1 fe1 =>
+              ∃z. peg_eval G (i0, choicel t) z ∧
+                  case z of
+                    Success i r eo =>
+                      x = Success i r (optmax MAXerr (SOME(fl1,fe1)) eo)
+                  | Failure fl2 fe2 =>
+                      x = UNCURRY Failure (MAXerr (fl1,fe1) (fl2,fe2))
 Proof
   simp[choicel_def, SimpLHS, Once peg_eval_cases] >>
-  dsimp[FORALL_result, resultmap_EQ_Success, rmax_EQ_Success] >>
-  conj_tac >- metis_tac[] >>
-  dsimp[EXISTS_result, AllCaseEqs()] >> metis_tac[]
+  dsimp[FORALL_result, EXISTS_result] >>
+  metis_tac[]
 QED
 
 Theorem peg_eval_rpt:
   peg_eval G (i0, rpt s f) x ⇔
-      ∃i l. peg_eval_list G (i0,s) (i,l) ∧ x = Success i (f l)
+    ∃i l err. peg_eval_list G (i0,s) (i,l,err) ∧ x = Success i (f l) (SOME err)
 Proof simp[Once peg_eval_cases, SimpLHS] >> metis_tac[]
 QED
 
 val peg_eval_list = Q.store_thm(
   "peg_eval_list",
-  `peg_eval_list G (i0, e) (i, r) ⇔
-     ∃fr. peg_eval G (i0, e) fr ∧ isFailure fr ∧ i = i0 ∧ r = [] ∨
-     (∃i1 rh rt.
-        peg_eval G (i0, e) (Success i1 rh) ∧
-        peg_eval_list G (i1, e) (i, rt) ∧ r = rh::rt)`,
+  `peg_eval_list G (i0, e) (i, r, err) ⇔
+     (∃fl fe. peg_eval G (i0, e) (Failure fl fe) ∧ i = i0 ∧ r = [] ∧
+             err = (fl,fe)) ∨
+     (∃i1 rh rt eo0.
+        peg_eval G (i0, e) (Success i1 rh eo0) ∧
+        peg_eval_list G (i1, e) (i, rt, err) ∧ r = rh::rt)`,
   simp[Once peg_eval_cases, SimpLHS] >> metis_tac[]);
 
 Theorem pegfail_empty[simp]:
